src/Manifest_Compiler.v
@@ -1,7 +1,7 @@
 (* Implementation of the Manifest Compiler.
     Takes a Manifest + AM_Library to an AM_Config.  *)
 
-Require Import Maps AbstractedTypes EqClass Term_Defs_Core Manifest_Admits Manifest
+Require Import Maps ID_Type EqClass Term_Defs_Core Manifest_Admits Manifest
   ErrorStMonad_Coq Term_Defs Interface_Types CvmJson_Interfaces Manifest_Set
   IO_Stubs.
 
