src/Manifest_Union.v
@@ -1,6 +1,6 @@
 (* Defining union operations for Manifests and Manifest Environments. *)
 
-Require Import AbstractedTypes Term_Defs_Core Maps String
+Require Import ID_Type Term_Defs_Core Maps String
   Term_Defs Manifest_Admits EqClass ErrorStMonad_Coq.
 
 Require Import Manifest Manifest_Set EnvironmentM.
